src/Util/Mat.v
@@ -1,60 +1,63 @@
-Require Import CoqChess.Util.Dec.
-Require Import CoqChess.Util.Fin.
-Require Import CoqChess.Util.Vec.
+Require Import Games.Util.Dec.
+Require Import Games.Util.Fin.
+Require Import Games.Util.Vec.
 
 Definition Mat (X : Type) (m n : nat) : Type :=
   Vec (Vec X n) m.
 
-Definition fin_maccess {X} {m n} : Fin m -> Fin n
+Definition mreplicate {X} {m n} (x : X) : Mat X m n :=
+  vreplicate (vreplicate x).
+
+Definition maccess {X} {m n} : Fin m -> Fin n
   -> Mat X m n -> X :=
-  fun i j mat => fin_vaccess j (fin_vaccess i mat).
+  fun i j mat => vaccess j (vaccess i mat).
 
-Definition fin_mupdate {X} {m n} : Fin m -> Fin n
+Definition mupdate {X} {m n} : Fin m -> Fin n
   -> X -> Mat X m n -> Mat X m n :=
-  fun i j x mat => fin_vupdate i
-    (fin_vupdate j x (fin_vaccess i mat)) mat.
+  fun i j x mat => vupdate i
+    (vupdate j x (vaccess i mat)) mat.
 
-Lemma fin_maccess_fin_mupdate_eq {X} {m n} :
+Lemma maccess_mupdate_eq {X} {m n} :
   forall (i : Fin m) (j : Fin n) (mat : Mat X m n) (x : X),
-  fin_maccess i j (fin_mupdate i j x mat) = x.
+  maccess i j (mupdate i j x mat) = x.
 Proof.
-  unfold fin_maccess, fin_mupdate.
+  unfold maccess, mupdate.
   intros.
-  repeat rewrite fin_vaccess_fin_vupdate_eq; reflexivity.
+  repeat rewrite vaccess_vupdate_eq; reflexivity.
 Qed.
 
-Lemma fin_maccess_fin_mupdate_neq1 {X} {m n} :
+Lemma maccess_mupdate_neq1 {X} {m n} :
   forall (i1 i2 : Fin m) (j1 j2 : Fin n) (mat : Mat X m n) (x : X),
   i1 <> i2 ->
-  fin_maccess i1 j1 (fin_mupdate i2 j2 x mat) =
-  fin_maccess i1 j1 mat.
+  maccess i1 j1 (mupdate i2 j2 x mat) =
+  maccess i1 j1 mat.
 Proof.
-  unfold fin_maccess, fin_mupdate.
+  unfold maccess, mupdate.
   intros.
-  rewrite fin_vaccess_fin_vupdate_neq; auto.
+  rewrite vaccess_vupdate_neq; auto.
 Qed.
 
-Lemma fin_maccess_fin_mupdate_neq2 {X} {m n} :
+Lemma maccess_mupdate_neq2 {X} {m n} :
   forall (i : Fin m) (j1 j2 : Fin n) (mat : Mat X m n) (x : X),
   j1 <> j2 ->
-  fin_maccess i j1 (fin_mupdate i j2 x mat) =
-  fin_maccess i j1 mat.
+  maccess i j1 (mupdate i j2 x mat) =
+  maccess i j1 mat.
 Proof.
-  unfold fin_maccess, fin_mupdate.
+  unfold maccess, mupdate.
   intros.
-  rewrite fin_vaccess_fin_vupdate_eq.
-  apply fin_vaccess_fin_vupdate_neq; auto.
+  rewrite vaccess_vupdate_eq.
+  apply vaccess_vupdate_neq; auto.
 Qed.
 
-Lemma fin_maccess_fin_mupdate_neq {X} {m n} :
+Lemma maccess_mupdate_neq {X} {m n} :
   forall (i1 i2 : Fin m) (j1 j2 : Fin n) (mat : Mat X m n) (x : X),
   (i1, j1) <> (i2, j2) ->
-  fin_maccess i1 j1 (fin_mupdate i2 j2 x mat) =
-  fin_maccess i1 j1 mat.
+  maccess i1 j1 (mupdate i2 j2 x mat) =
+  maccess i1 j1 mat.
 Proof.
   intros.
   destruct (dec (P := i1 = i2)).
   - rewrite e.
-    rewrite fin_maccess_fin_mupdate_neq2; congruence.
-  - rewrite fin_maccess_fin_mupdate_neq1; auto.
+    rewrite maccess_mupdate_neq2; congruence.
+  - rewrite maccess_mupdate_neq1; auto.
 Qed.
