src/Util/Vec.v
@@ -1,8 +1,8 @@
 Require Import Arith.
 Import Nat.
 
-Require Import CoqChess.Util.Fin.
-Require Import CoqChess.Util.UIP.
+Require Import Games.Util.Fin.
+Require Import Games.Util.UIP.
 
 Fixpoint Vec (X : Type) (n : nat) : Type :=
   match n with
@@ -10,84 +10,63 @@ Fixpoint Vec (X : Type) (n : nat) : Type :=
   | S m => X * Vec X m
   end.
 
-Fixpoint access {X} {n} : forall i, i < n -> Vec X n -> X :=
+Fixpoint vreplicate {X} {n} (x : X) : Vec X n :=
   match n with
-  | 0 => fun i pf =>
-    match nlt_0_r i pf with
+  | 0 => tt
+  | S m => (x, vreplicate x)
+  end.
+
+Fixpoint vaccess {X} {n} : Fin n -> Vec X n -> X :=
+  match n with
+  | 0 => fun e =>
+    match e with
     end
   | S m => fun i =>
     match i with
-    | 0 => fun _ => fst
-    | S j => fun pf v => access j (lt_S_n j m pf) (snd v)
+    | inl _ => fst
+    | inr j => fun v => vaccess j (snd v)
     end
   end.
 
-Definition fin_vaccess {X} {n} : Fin n -> Vec X n -> X :=
-  fun '(existT _ i pf) => access i pf.
-
-Fixpoint update {X} {n} : forall i, i < n -> X -> Vec X n -> Vec X n :=
+Fixpoint vupdate {X} {n} : Fin n -> X -> Vec X n -> Vec X n :=
   match n with
-  | 0 => fun i pf =>
-    match nlt_0_r i pf with
+  | 0 => fun e =>
+    match e with
     end
   | S m => fun i =>
     match i with
-    | 0 => fun _ x v => (x, snd v)
-    | S j => fun pf x v => (fst v, update j
-      (lt_S_n j m pf) x (snd v))
+    | inl _ => fun x v => (x, snd v)
+    | inr j => fun x v => (fst v, vupdate j x (snd v))
     end
   end.
 
-Definition fin_vupdate {X} {n} : Fin n -> X -> Vec X n -> Vec X n :=
-  fun '(existT _ i pf) => update i pf.
-
-Lemma access_update_eq : forall {X} {n}
-  i (pf : i < n) v (x : X),
-  access i pf (update i pf x v) = x.
-Proof.
-  intro X.
-  induction n; intros.
-  { inversion pf. }
-  { destruct i; simpl; auto. }
-Qed.
-
-Lemma access_update_neq : forall {X} {n}
-  i (pf : i < n) j (pf' : j < n) v (x : X),
-  i <> j -> access i pf (update j pf' x v)
-  = access i pf v.
-Proof.
-  intro X.
-  induction n; intros.
-  { inversion pf. }
-  { destruct i, j; auto.
-    { elim H; auto. }
-    { simpl.
-      apply IHn; auto.
-    }
-  }
-Qed.
-
-Lemma fin_vaccess_fin_vupdate_eq : forall {X} {n}
+Lemma vaccess_vupdate_eq : forall {X} {n}
   (i : Fin n) v (x : X),
-  fin_vaccess i (fin_vupdate i x v) = x.
+  vaccess i (vupdate i x v) = x.
 Proof.
-  intros.
-  unfold fin_vaccess, fin_vupdate.
-  destruct i.
-  apply access_update_eq.
+  intros X n i v x.
+  induction n.
+  - destruct i.
+  - destruct i as [[]|j].
+    + reflexivity.
+    + simpl.
+      apply IHn.
 Qed.
 
-Lemma fin_vaccess_fin_vupdate_neq : forall {X} {n}
+Lemma vaccess_vupdate_neq : forall {X} {n}
   (i j : Fin n) v (x : X), i <> j ->
-  fin_vaccess i (fin_vupdate j x v) = fin_vaccess i v.
+  vaccess i (vupdate j x v) = vaccess i v.
 Proof.
-  intros.
-  unfold fin_vaccess, fin_vupdate.
-  destruct i as [i Hi].
-  destruct j as [j Hj].
-  apply access_update_neq.
-  intro pf.
-  apply H.
-  destruct pf.
-  f_equal; apply UIP.
+  intros X n i j v x ij_neq.
+  induction n.
+  - destruct i.
+  - destruct i as [[]|i'];
+    destruct j as [[]|j'].
+    + now elim ij_neq.
+    + reflexivity.
+    + reflexivity.
+    + simpl.
+      apply IHn.
+      intro; elim ij_neq.
+      congruence.
 Qed.
