src/Game/TB.v
@@ -1,0 +1,842 @@
+Require Import Lia.
+Require Import List.
+Import ListNotations.
+
+Require Import Games.Game.Game.
+Require Import Games.Game.Player.
+Require Import Games.Game.Draw.
+Require Import Games.Game.Win.
+
+Require Import Games.Util.TBLoop.
+Require Import Games.Util.StringMap.
+Require Import Games.Util.Show.
+Require Import Games.Util.Dec.
+
+Class FinGame (G : Game) : Type := {
+  enum_states : list (GameState G);
+  enum_wins : Player -> list (GameState G);
+
+  enum_states_correct : forall s, In s enum_states;
+  enum_wins_correct1 : forall s pl,
+    In s (enum_wins pl) -> atomic_res s = Some (Win pl);
+  enum_wins_correct2 : forall s pl,
+    atomic_res s = Some (Win pl) -> In s (enum_wins pl)
+  }.
+
+Class NiceGame (G : Game) : Prop := {
+  atomic_win_opp : forall (s : GameState G) pl,
+    atomic_res s = Some (Win pl) ->
+    to_play s = opp pl
+  }.
+
+Class Reversible (G : Game) : Type := {
+  enum_preds : GameState G -> list (GameState G);
+
+  enum_preds_correct1 : forall s s' : GameState G,
+    In s (enum_preds s') -> exists m, exec_move s m = s';
+  enum_preds_correct2 : forall (s : GameState G)
+    (m : Move s), In s (enum_preds (exec_move s m))
+  }.
+
+Section TB.
+
+Context {G : Game}.
+Context `{FinGame G}.
+Context `{NiceGame G}.
+Context `{Reversible G}.
+Context `{Show (GameState G)}.
+Context `{forall s : GameState G, Discrete (Move s)}.
+
+Context {M : Type -> Type}.
+Context `{StringMap M}.
+
+Inductive Step :=
+  | Eloise : Step
+  | Abelard : Step.
+
+Definition switch : Step -> Step :=
+  fun s =>
+    match s with
+    | Eloise => Abelard
+    | Abelard => Eloise
+    end.
+
+Definition step_player : Step -> Player -> Player :=
+  fun s =>
+    match s with
+    | Eloise => fun pl => pl
+    | Abelard => opp
+    end.
+
+Record TB : Type := {
+  curr : nat;
+  last_step : Step;
+
+  white_positions : M (Player * nat);
+  black_positions : M (Player * nat);
+
+  last_white_positions : list (GameState G);
+  last_black_positions : list (GameState G)
+  }.
+
+Definition tb_lookup (tb : TB) (s : GameState G) : option (Player * nat) :=
+  match to_play s with
+  | White => str_lookup s (white_positions tb)
+  | Black => str_lookup s (black_positions tb)
+  end.
+
+Definition tag (winner : Player) (n : nat) (s : GameState G) :=
+  (s, (winner, n)).
+
+Definition add_positions (m : M (Player * nat)) (winner : Player) (n : nat)
+  (ps : list (GameState G)) : M (Player * nat) :=
+  str_adds (map (tag winner n) ps) m.
+
+Fixpoint filter_Nones {X Y} (f : X -> option Y) (xs : list X) : list X :=
+  match xs with
+  | [] => []
+  | x :: xs' =>
+    match f x with
+    | None => x :: filter_Nones f xs'
+    | Some _ => filter_Nones f xs'
+    end
+  end.
+
+Definition eloise_step (tb : TB) (pl : Player) : list (GameState G) :=
+  let prev :=
+    match pl with
+    | White => last_black_positions tb
+    | Black => last_white_positions tb
+    end in
+  let m :=
+    match pl with
+    | White =>
+        add_positions
+          (white_positions tb)
+          (step_player (last_step tb) White)
+          (curr tb)
+          (last_white_positions tb)
+    | Black =>
+        add_positions
+          (black_positions tb)
+          (step_player (last_step tb) Black)
+          (curr tb)
+          (last_black_positions tb)
+    end in
+  let candidates := concat (map enum_preds prev) in
+  let candidates' :=
+    filter_Nones (fun s => str_lookup s m) candidates in
+  nodup Show_dec candidates'.
+
+Definition abelard_step (tb : TB) (pl : Player) : list (GameState G) :=
+  let prev :=
+    match pl with
+    | White => last_black_positions tb
+    | Black => last_white_positions tb
+    end in
+  let m :=
+    match pl with
+    | White =>
+        add_positions
+          (white_positions tb)
+          (step_player (last_step tb) White)
+          (curr tb)
+          (last_white_positions tb)
+    | Black =>
+        add_positions
+          (black_positions tb)
+          (step_player (last_step tb) Black)
+          (curr tb)
+          (last_black_positions tb)
+    end in
+  let m' :=
+    match pl with
+    | Black =>
+        add_positions
+          (white_positions tb)
+          (step_player (last_step tb) White)
+          (curr tb)
+          (last_white_positions tb)
+    | White =>
+        add_positions
+          (black_positions tb)
+          (step_player (last_step tb) Black)
+          (curr tb)
+          (last_black_positions tb)
+    end in
+  let candidates := concat (map enum_preds prev) in
+  let candidates' :=
+    filter_Nones (fun s => str_lookup s m) candidates in
+  let candidates'' := filter
+    (fun s => forallb (fun m =>
+      match str_lookup (exec_move s m) m' with
+      | Some (pl',_) => player_eqb (opp pl) pl'
+      | None => false
+      end) (enum_moves s)) candidates' in
+  nodup Show_dec candidates''.
+
+Definition TB_init : TB := {|
+  curr := 0;
+  last_step := Abelard;
+
+  white_positions := empty;
+  black_positions := empty;
+
+  last_white_positions := nodup Show_dec (enum_wins Black);
+  last_black_positions := nodup Show_dec (enum_wins White);
+  |}.
+
+Definition TB_step (tb : TB) : TB := {|
+  curr := S (curr tb);
+  last_step := switch (last_step tb);
+
+  white_positions := add_positions
+    (white_positions tb)
+    (step_player (last_step tb) White)
+    (curr tb)
+    (last_white_positions tb);
+  black_positions := add_positions
+    (black_positions tb)
+    (step_player (last_step tb) Black)
+    (curr tb)
+    (last_black_positions tb);
+
+  last_white_positions :=
+    match last_step tb with
+    | Eloise => abelard_step tb White
+    | Abelard => eloise_step tb White
+    end;
+  last_black_positions :=
+    match last_step tb with
+    | Eloise => abelard_step tb Black
+    | Abelard => eloise_step tb Black
+    end
+  |}.
+
+Definition num_left (tb : TB) : nat :=
+  length enum_states -
+  size (white_positions tb) -
+  size (black_positions tb).
+
+Definition num_left_decr : forall tb,
+  num_left (TB_step tb) <= num_left tb.
+Proof.
+  unfold num_left.
+  intros []; simpl.
+  unfold add_positions.
+  pose proof (str_size_adds_le
+    (map (tag (step_player last_step0 White) curr0) last_white_positions0)
+    white_positions0).
+  pose proof (str_size_adds_le
+    (map (tag (step_player last_step0 Black) curr0) last_black_positions0)
+    black_positions0).
+  lia.
+Qed.
+
+Definition TB_loop_data : loop_data TB := {|
+  measure := num_left;
+  step := TB_step;
+  step_measure := num_left_decr
+  |}.
+
+Definition TB_final : TB :=
+  loop TB_loop_data TB_init.
+
+Definition respects_atomic_wins (tb : TB) : Prop := forall s pl,
+  atomic_res s = Some (Win pl) ->
+  tb_lookup tb s = Some (pl, 0).
+
+Record TB_valid (tb : TB) : Type := {
+
+  win_tb : forall {s pl} (w : win pl s),
+    depth w < curr tb -> {n : nat & tb_lookup tb s = Some (pl, n)};
+
+  tb_win : forall {s pl n},
+    tb_lookup tb s = Some (pl, n) ->
+    win pl s;
+
+  tb_win_depth : forall {s pl n} (pf : tb_lookup tb s = Some (pl, n)),
+    depth (tb_win pf) = n;
+
+  tb_win_sat : forall {s pl n} (pf : tb_lookup tb s = Some (pl, n)),
+    saturated (tb_win pf);
+
+  win_last_white_positions : forall {s pl} (w : win pl s), to_play s = White ->
+    depth w = curr tb -> In s (last_white_positions tb);
+
+  last_white_positions_win : forall {s}, In s (last_white_positions tb) ->
+    win (step_player (last_step tb) White) s;
+
+  last_white_positions_win_depth : forall {s} (pf : In s (last_white_positions tb)),
+    depth (last_white_positions_win pf) = curr tb;
+
+  win_last_black_positions : forall {s pl} (w : win pl s), to_play s = Black ->
+    depth w = curr tb -> In s (last_black_positions tb);
+
+  tb_respects_atomic_wins : curr tb = 0 \/ respects_atomic_wins tb;
+
+  last_white_positions_NoDup : NoDup (last_white_positions tb);
+
+  last_black_positions_NoDup : NoDup (last_black_positions tb);
+
+  last_white_positions_disj : forall s, In s (last_white_positions tb) -> str_lookup s (white_positions tb) = None;
+
+  last_black_positions_disj : forall s, In s (last_black_positions tb) -> str_lookup s (black_positions tb) = None;
+
+  sizes_never_exceed :
+    size (white_positions tb) +
+    size (black_positions tb) +
+    length (last_white_positions tb) +
+    length (last_black_positions tb) <= length enum_states;
+
+  }.
+
+(* Lemma win_tb_TB_init : forall s pl (w : win pl s),
+    depth w < curr TB_init -> {n : nat & tb_lookup TB_init s = Some (pl, n)}.
+Proof.
+  unfold TB_init; simpl; lia.
+Defined. *)
+
+Lemma tb_win_TB_init :  forall s pl n,
+  tb_lookup TB_init s = Some (pl, n) ->
+  win pl s.
+Proof.
+  unfold TB_init, tb_lookup; simpl.
+  intros s pl n Hs.
+  destruct (to_play s);
+  now rewrite str_lookup_empty in Hs.
+Defined.
+
+Lemma last_white_positions_win_TB_init : forall s,
+  In s (last_white_positions TB_init) ->
+  win (step_player (last_step TB_init) White) s.
+Proof.
+  intros.
+  apply atom_win.
+  simpl.
+  apply enum_wins_correct1.
+  simpl in H5.
+  now rewrite nodup_In in H5.
+Defined.
+
+Definition disj {X} (xs ys : list X) : Prop :=
+  forall x, In x xs -> ~ In x ys.
+
+Lemma NoDup_app {X} : forall (xs ys : list X),
+  NoDup xs -> NoDup ys -> disj xs ys -> NoDup (xs ++ ys).
+Proof.
+  induction xs as [|x xs']; intros ys nd_xs nd_ys d_xs_ys.
+  - exact nd_ys.
+  - simpl.
+    constructor.
+    + rewrite in_app_iff.
+      intros [in_x_xs'|in_x_ys].
+      * now inversion nd_xs.
+      * apply (d_xs_ys x); [now left|auto].
+    + apply IHxs'; auto.
+      * now inversion nd_xs.
+      * intros y in_y_xs' in_y_ys.
+        apply (d_xs_ys y); [now right|auto].
+Qed.
+
+Lemma TB_init_valid : TB_valid TB_init.
+  refine {|
+    win_tb := _;
+    tb_win := tb_win_TB_init;
+    tb_win_depth := _;
+    tb_win_sat := _;
+    win_last_white_positions := _;
+    last_white_positions_win := last_white_positions_win_TB_init;
+    last_white_positions_win_depth := _;
+    win_last_black_positions := _;
+    tb_respects_atomic_wins := _;
+    last_white_positions_NoDup := _;
+    last_black_positions_NoDup := _;
+    last_white_positions_disj := _;
+    last_black_positions_disj := _;
+    sizes_never_exceed := _;
+  |}.
+Proof.
+  (* win_tb *)
+  - unfold TB_init; simpl; lia.
+  (* tb_win_depth *)
+  - intros.
+    cut False; [tauto|].
+    unfold tb_lookup in pf.
+    destruct (to_play s) eqn:s_play; simpl in pf;
+    now rewrite str_lookup_empty in pf.
+  (* tb_win_sat *)
+  - intros.
+    cut False; [tauto|].
+    unfold tb_lookup in pf.
+    destruct (to_play s) eqn:s_play; simpl in pf;
+    now rewrite str_lookup_empty in pf.
+  (* win_last_white_positions *)
+  - intros s pl w s_play w_depth.
+    simpl in *.
+    rewrite nodup_In.
+    apply enum_wins_correct2.
+    destruct w.
+    + rewrite (atomic_win_opp _ _ e) in s_play.
+      now destruct pl.
+    + now simpl in w_depth.
+    + now simpl in w_depth.
+  (* last_white_positions_win_depth *)
+  - now intros.
+  (* win_last_black_positions *)
+  - intros s pl w s_play w_depth.
+    simpl in *.
+    rewrite nodup_In.
+    apply enum_wins_correct2.
+    destruct w.
+    + rewrite (atomic_win_opp _ _ e) in s_play.
+      now destruct pl.
+    + now simpl in w_depth.
+    + now simpl in w_depth.
+  (* tb_respects_atomic_wins *)
+  - now left.
+  (* last_white_positions_NoDup *)
+  - apply NoDup_nodup.
+  (* last_black_positions_NoDup *)
+  - apply NoDup_nodup.
+  (* last_white_positions_disj *)
+  - intros; apply str_lookup_empty.
+  (* last_black_positions_disj *)
+  - intros; apply str_lookup_empty.
+  (* sizes_never_exceed *)
+  - simpl; rewrite size_empty; simpl.
+    rewrite <- app_length.
+    apply NoDup_incl_length.
+    + apply NoDup_app.
+      * apply NoDup_nodup.
+      * apply NoDup_nodup.
+      * intros s s_b s_w.
+        rewrite nodup_In in s_b, s_w.
+        pose proof (enum_wins_correct1 _ _ s_b);
+        pose proof (enum_wins_correct1 _ _ s_w);
+        congruence.
+    + intros s _.
+      apply enum_states_correct.
+Defined.
+
+Lemma TB_step_valid : forall tb, TB_valid tb
+  -> TB_valid (TB_step tb).
+Proof.
+Admitted.
+
+Definition TB_validity_data : validity_data TB_loop_data.
+Proof.
+  refine ( {|
+  valid := TB_valid;
+  step_valid := _
+  |} ).
+  exact TB_step_valid.
+Defined.
+
+Lemma TB_final_valid : TB_valid TB_final.
+Proof.
+  exact (loop_valid _
+    TB_validity_data _ TB_init_valid).
+Defined.
+
+Lemma iter_curr : forall k,
+  curr (Nat.iter k TB_step TB_init) = k.
+Proof.
+  induction k.
+  - reflexivity.
+  - simpl; congruence.
+Qed.
+
+Lemma In_length_pos {X} (xs : list X) : forall x, In x xs ->
+  length xs > 0.
+Proof.
+  destruct xs; intros y HIn.
+  - destruct HIn.
+  - simpl; lia.
+Qed.
+
+Lemma num_left_lt : forall tb (s : GameState G) pl
+  (w : win pl s), TB_valid tb -> depth w = curr tb ->
+  num_left (step TB_loop_data tb) < num_left tb.
+Proof.
+  intros.
+  unfold num_left.
+  simpl.
+  unfold add_positions.
+  rewrite str_size_adds.
+  - rewrite str_size_adds.
+    + repeat rewrite map_length.
+      pose (E := length enum_states).
+      pose (W := length (last_white_positions tb)).
+      pose (SW := size (white_positions tb)).
+      pose (B := length (last_black_positions tb)).
+      pose (SB := size (black_positions tb)).
+      fold E W SW B SB.
+      assert (SW + SB + W + B <= E).
+      { apply sizes_never_exceed; auto. }
+      destruct (to_play s) eqn:s_play.
+      * assert (W > 0).
+        { unfold W.
+          apply (In_length_pos _ s).
+          eapply win_last_white_positions; eauto.
+        }
+        lia.
+      * assert (B > 0).
+        { unfold W.
+          apply (In_length_pos _ s).
+          eapply win_last_black_positions; eauto.
+        }
+        lia.
+    + rewrite map_map.
+      unfold tag.
+      simpl.
+      rewrite map_id.
+      apply last_black_positions_NoDup; auto.
+    + rewrite map_map.
+      unfold tag.
+      simpl.
+      rewrite map_id.
+      apply last_black_positions_disj; auto.
+  - rewrite map_map.
+    unfold tag.
+    simpl.
+    rewrite map_id.
+    apply last_white_positions_NoDup; auto.
+  - rewrite map_map.
+    unfold tag.
+    simpl.
+    rewrite map_id.
+    apply last_white_positions_disj; auto.
+Qed.
+
+Lemma win_TB_final_lookup : forall s pl,
+  win pl s -> {n : nat & tb_lookup TB_final s = Some (pl, n)}.
+Proof.
+  intros s pl w.
+  destruct (win_tb TB_final TB_final_valid w).
+  - destruct (loop_iter TB_loop_data TB_init) as [k Hk].
+    unfold TB_final; rewrite Hk.
+    rewrite iter_curr.
+    destruct (Compare_dec.le_lt_dec k (depth w)); [|auto].
+    destruct (depth_lower _ _ l) as [s' [w' w'_depth]].
+    pose proof (loop_measure TB_loop_data TB_init).
+    rewrite Hk in H5.
+    simpl in H5.
+    assert (num_left (TB_step (Nat.iter k TB_step TB_init)) <
+      num_left (Nat.iter k TB_step TB_init));
+      [|lia].
+    eapply num_left_lt.
+    + apply (iter_step_valid TB_loop_data TB_validity_data).
+      exact TB_init_valid.
+    + rewrite iter_curr. exact w'_depth.
+  - exists x.
+    exact e.
+Defined.
+
+Theorem TB_final_lookup_mate : forall s pl n,
+  tb_lookup TB_final s = Some (pl, n) ->
+  mate pl s n.
+Proof.
+  intros.
+  destruct TB_final_valid.
+  exists (tb_win0 _ _ _ H5).
+  split.
+  - apply tb_win_depth0.
+  - apply saturated_minimal.
+    apply tb_win_sat0.
+Defined.
+
+Theorem mate_TB_final_lookup : forall s pl n,
+  mate pl s n ->
+  tb_lookup TB_final s = Some (pl, n).
+Proof.
+  intros s pl n [w [w_d w_m]].
+  destruct (win_TB_final_lookup _ _ w) as [m Hm].
+  destruct (TB_final_lookup_mate _ _ _ Hm) as
+    [w' [w'_d w'_m]].
+  cut (m = n); [congruence|].
+  pose (w_m w').
+  pose (w'_m w).
+  lia.
+Qed.
+
+Lemma None_or_all_Some {X Y} (f : X -> option Y) (xs : list X) :
+  { x : X & f x = None } +
+  { ys : list Y & map f xs = map Some ys }.
+Proof.
+  induction xs as [|x xs'].
+  - right.
+    exists [].
+    reflexivity.
+  - destruct (f x) eqn:fx.
+    + destruct IHxs' as [[x' Hx']| [ys Hys]].
+      * left; now exists x'.
+      * right; exists (y :: ys); simpl; congruence.
+    + left; now exists x.
+Defined.
+
+Lemma map_fg_lemma {X Y Z} `{Discrete Y} {f : X -> Z} {g : Y -> Z} :
+  forall {xs ys}, map f xs = map g ys -> 
+  forall y, In y ys -> {x : X & In x xs /\ f x = g y}.
+Proof.
+  induction xs as [|x xs']; intros ys pf y Hy.
+  - destruct ys; [destruct Hy|inversion pf].
+  - destruct ys; [inversion pf|].
+    destruct (eq_dec y0 y).
+    + exists x; split.
+      * now left.
+      * inversion pf; congruence.
+    + inversion pf.
+      destruct (IHxs' _ H8 y).
+      * destruct Hy; [contradiction|auto].
+      * exists x0; split; [now right| tauto].
+Defined.
+
+Lemma forallb_false {X} (p : X -> bool) (xs : list X) :
+  forallb p xs = false -> {x : X & In x xs /\ p x = false}.
+Proof.
+  induction xs as [|x xs']; simpl; intros pf.
+  - discriminate.
+  - destruct (p x) eqn:px.
+    + destruct (IHxs' pf) as [x' [Hx'1 Hx'2]].
+      exists x'; tauto.
+    + exists x; tauto.
+Defined.
+
+Lemma forallb_true {X} (p : X -> bool) (xs : list X) :
+  forallb p xs = true -> forall x, In x xs -> p x = true.
+Proof.
+  induction xs as [|x' xs']; intros Hpxs x Hx.
+  - destruct Hx.
+  - destruct Hx; subst; simpl in *.
+    + destruct (p x); [reflexivity|discriminate].
+    + destruct (p x'); [simpl in *|discriminate].
+      now apply IHxs'.
+Qed.
+
+Lemma map_tag_functional : forall pl n ps,
+  AL.functional (map (tag pl n) ps).
+Proof.
+  intros pl n ps.
+  intros s [q1 k] [q2 l] Hq1 Hq2.
+  rewrite in_map_iff in Hq1, Hq2.
+  destruct Hq1 as [t [Ht _]].
+  destruct Hq2 as [u [Hu _]].
+  unfold tag in Ht, Hu.
+  congruence.
+Qed.
+
+(* (* Definition respects_atomic_wins (tb : TB) : Prop :=
+  forall s pl, atomic_res s = Some (Win pl) ->
+  tb_lookup tb s = Some (pl, 0). *) *)
+
+Lemma respects_atomic_wins_step_1 : respects_atomic_wins (TB_step TB_init).
+Proof.
+  intros s pl s_res.
+  unfold TB_step, TB_init, tb_lookup; simpl.
+  destruct (to_play s) eqn:s_play.
+  - unfold add_positions.
+    apply str_lookup_adds.
+    + apply map_tag_functional.
+    + rewrite in_map_iff.
+      rewrite (atomic_win_opp s pl s_res) in s_play.
+      destruct pl; [discriminate|].
+      exists s; split; [reflexivity|].
+      rewrite nodup_In.
+      now apply enum_wins_correct2.
+  - unfold add_positions.
+    apply str_lookup_adds.
+    + apply map_tag_functional.
+    + rewrite in_map_iff.
+      rewrite (atomic_win_opp s pl s_res) in s_play.
+      destruct pl; [|discriminate].
+      exists s; split; [reflexivity|].
+      rewrite nodup_In.
+      now apply enum_wins_correct2.
+Qed.
+
+(** TODO : use in step proof *)
+(* Lemma respects_atomic_wins_step : forall tb, TB_valid tb -> respects_atomic_wins tb ->
+  respects_atomic_wins (TB_step tb).
+Proof.
+  intros tb tb_v Htb s pl s_res.
+  unfold TB_step, tb_lookup; simpl.
+  destruct (to_play s) eqn:s_play; unfold add_positions.
+  - rewrite str_lookup_adds_nIn.
+    + pose proof (Htb s pl s_res) as Htb.
+      unfold tb_lookup in Htb.
+      now rewrite s_play in Htb.
+    + rewrite in_map_iff.
+      intros [[? [pl' n']] [? Hs]].
+      simpl in *; subst.
+      rewrite in_map_iff in Hs.
+      destruct Hs as [s' [Hs'1 Hs'2]].
+      unfold tag in Hs'1.
+      inversion Hs'1; subst.
+      pose (Htb s _ s_res).
+Admitted. *)
+
+Lemma TB_final_respects_atomic_wins :
+  respects_atomic_wins TB_final.
+Proof.
+  destruct (tb_respects_atomic_wins TB_final).
+  - apply TB_final_valid.
+  - destruct (loop_iter TB_loop_data TB_init) as [k Hk].
+    unfold TB_final in H5.
+    rewrite Hk in H5.
+    rewrite iter_curr in H5.
+    subst; simpl in *.
+    pose proof (loop_measure TB_loop_data TB_init) as Hmeasure.
+    simpl in Hmeasure.
+    rewrite Hk in Hmeasure.
+    unfold num_left in Hmeasure.
+    simpl in Hmeasure.
+    rewrite size_empty in Hmeasure.
+    unfold add_positions in Hmeasure.
+    intros s pl s_res.
+    assert (length enum_states > 0).
+    { apply (In_length_pos _ s).
+      apply enum_states_correct.
+    }
+    destruct (to_play s) eqn:s_play.
+    + assert (In (s, (Black, 0)) (map (tag Black 0) (nodup Show_dec (enum_wins Black)))) as Hs.
+      { rewrite in_map_iff.
+        exists s; split; [reflexivity|].
+        rewrite nodup_In.
+        erewrite atomic_win_opp in s_play; [|exact s_res].
+        apply enum_wins_correct2; now destruct pl.
+      }
+      pose proof (str_adds_ne_pos (map (tag Black 0) (nodup Show_dec (enum_wins Black)))
+        s (Black, 0) Hs); lia.
+    + assert (In (s, (White, 0)) (map (tag White 0) (nodup Show_dec (enum_wins White)))) as Hs.
+      { rewrite in_map_iff.
+        exists s; split; [reflexivity|].
+        rewrite nodup_In.
+        erewrite atomic_win_opp in s_play; [|exact s_res].
+        apply enum_wins_correct2; now destruct pl.
+      }
+      pose proof (str_adds_ne_pos (map (tag White 0) (nodup Show_dec (enum_wins White)))
+        s (White, 0) Hs); lia.
+  - auto.
+Qed.
+
+Lemma TB_lookup_None : forall s,
+  tb_lookup TB_final s = None ->
+  (atomic_res s = Some Draw) +
+  (atomic_res s = None) * { m : Move s & tb_lookup TB_final (exec_move s m) = None }.
+Proof.
+  intros.
+  destruct atomic_res eqn:s_res.
+  - destruct r.
+    + erewrite TB_final_respects_atomic_wins in H5;
+        [congruence|eauto].
+    + left; reflexivity.
+  - right; split; [reflexivity|].
+    destruct (None_or_all_Some
+      (fun m => tb_lookup TB_final (exec_move s m))
+      (enum_moves s)) as [[m Hm]|[ps Hps]].
+    + now exists m.
+    + destruct (forallb
+        (fun p => player_eqb (fst p) (opp (to_play s))) ps) eqn:Hps2.
+      * cut (win (opp (to_play s)) s); [intro w;
+           destruct (win_TB_final_lookup _ _ w); congruence|].
+        apply abelard_win; [auto | now rewrite opp_invol|].
+        intro m.
+        pose proof (forallb_true _ _ Hps2).
+        symmetry in Hps.
+        destruct (map_fg_lemma Hps m (enum_all m)) as
+          [[pl n] [HIn Htb]].
+        symmetry in Htb.
+        destruct (TB_final_lookup_mate _ _ _ Htb) as [w _].
+        eapply (tb_win TB_final TB_final_valid).
+        rewrite <- (player_eqb_true _ _ (H6 _ HIn)); simpl.
+        exact Htb.
+      * destruct (forallb_false _ _ Hps2) as [[pl n] [HIn Heqb]].
+        simpl in *.
+        pose proof (player_eqb_false _ _ Heqb) as pf.
+        rewrite opp_invol in pf.
+        destruct (map_fg_lemma Hps _ HIn) as [m [_ tb_m]].
+        pose (w := tb_win TB_final TB_final_valid tb_m).
+        symmetry in pf.
+        pose (w' := eloise_win s_res pf m w).
+        destruct (win_TB_final_lookup _ _ w') as [k tb_s].
+        congruence.
+Defined.
+
+Theorem TB_final_lookup_draw : forall s,
+  tb_lookup TB_final s = None ->
+  draw s.
+Proof.
+  cofix d.
+  intros s tb_s.
+  destruct (TB_lookup_None s tb_s) as
+    [|[s_res [m tb_sm]]].
+  - now apply atom_draw.
+  - eapply (play_draw s _ eq_refl s_res).
+    + clear m tb_sm.
+      intro m.
+      destruct (tb_lookup TB_final (exec_move s m)) eqn:tb_sm.
+      * destruct p as [pl n].
+        destruct (player_id_or_opp_r_t (to_play s) pl) as [pf|pf].
+        ** pose (w := tb_win TB_final TB_final_valid tb_sm).
+           pose (eloise_win s_res pf _ w) as w'.
+           destruct (win_TB_final_lookup _ _ w').
+           congruence.
+        ** right.
+           rewrite pf.
+           rewrite opp_invol.
+           eapply tb_win; [|eauto].
+           exact TB_final_valid.
+      * left.
+        apply d.
+        exact tb_sm.
+    + apply d.
+      exact tb_sm.
+Defined.
+
+Theorem draw_TB_final_lookup : forall s,
+  draw s ->
+  tb_lookup TB_final s = None.
+Proof.
+  intros s d.
+  destruct (tb_lookup TB_final s) eqn:tb_s; [|reflexivity].
+  destruct p as [pl n].
+  destruct (TB_final_lookup_mate s pl n tb_s) as
+    [w _].
+  elim (win_not_draw _ _ w d).
+Qed.
+
+End TB.
+
+Record CorrectTablebase (M : Type -> Type) `{StringMap M}
+  (G : Game) `{Show (GameState G)} := {
+
+  tb : TB (G := G) (M := M);
+
+  tb_lookup_mate : forall s pl n,
+    tb_lookup tb s = Some (pl, n) ->
+    mate pl s n;
+  mate_tb_lookup : forall s pl n,
+    mate pl s n ->
+    tb_lookup tb s = Some (pl, n);
+
+  tb_lookup_draw : forall s,
+    tb_lookup tb s = None ->
+    draw s;
+
+  draw_tb_lookup : forall s,
+    draw s ->
+    tb_lookup tb s = None
+
+  }.
+
+Definition certified_TB {M} `{StringMap M}
+  {G} `{Show (GameState G)} `{FinGame G} `{Reversible G}
+  `{NiceGame G} `{forall s, Discrete (Move s)} :
+  CorrectTablebase M G := {|
+  tb := TB_final;
+  tb_lookup_mate := TB_final_lookup_mate;
+  mate_tb_lookup := mate_TB_final_lookup;
+  tb_lookup_draw := TB_final_lookup_draw;
+  draw_tb_lookup := draw_TB_final_lookup
+  |}.
