src/Util/AssocList.v
@@ -1,0 +1,95 @@
+Require Import List.
+Import ListNotations.
+
+Require Import Games.Util.Dec.
+
+Definition t (K V : Type) : Type :=
+  list (K * V).
+
+Definition empty {K V} : t K V := [].
+
+Fixpoint add {K V} `{Discrete K}
+  (k : K) (v : V) (ps : t K V) : t K V :=
+  match ps with
+  | [] => [(k,v)]
+  | (k',v') :: qs =>
+    match eq_dec k k' with
+    | left _ => (k,v) :: qs
+    | right _ => (k',v') :: add k v qs
+    end
+  end.
+
+Fixpoint lookup {K V} `{Discrete K}
+  (k : K) (ps : t K V) : option V :=
+  match ps with
+  | [] => None
+  | (k',v) :: qs =>
+    match eq_dec k k' with
+    | left _ => Some v
+    | right _ => lookup k qs
+    end
+  end.
+
+Definition size {K V} (ps : t K V) : nat :=
+  length ps.
+
+Lemma lookup_empty {K V} `{Discrete K} : forall k,
+  lookup k (empty : t K V) = None.
+Proof.
+  auto.
+Qed.
+
+Lemma lookup_add {K V} `{Discrete K} : forall (k : K) (v : V) m,
+  lookup k (add k v m) = Some v.
+Proof.
+  intros k v m.
+  induction m as [|[k' v'] m'].
+  - simpl; now destruct (eq_dec k k).
+  - simpl; destruct (eq_dec k k').
+    + simpl; now destruct (eq_dec k k).
+    + simpl; now destruct (eq_dec k k').
+Qed.
+
+Lemma lookup_add_neq {K V} `{Discrete K} : forall (k k' : K) (v : V) m,
+  k <> k' -> lookup k (add k' v m) = lookup k m.
+Proof.
+  intros k k' v m Hkk'.
+  induction m as [|[k'' v''] m'].
+  - simpl; now destruct (eq_dec k k').
+  - simpl; destruct (eq_dec k' k'').
+    + simpl; destruct (eq_dec k k'').
+      * congruence.
+      * now destruct (eq_dec k k').
+    + simpl; now rewrite IHm'.
+Qed.
+
+Lemma size_empty {K V} : size (empty : t K V) = 0.
+Proof.
+  reflexivity.
+Qed.
+
+Lemma size_add {K V} `{Discrete K} : forall (k : K) (v : V) m,
+  size (add k v m) =
+    match lookup k m with
+    | Some _ => size m
+    | None => S (size m)
+    end.
+Proof.
+  intros k v m.
+  induction m as [|[k' v'] m'].
+  - reflexivity.
+  - simpl.
+    destruct (eq_dec k k').
+    + reflexivity.
+    + simpl; destruct (lookup k m'); auto.
+Qed.
+
+Definition functional {K V} (ps : list (K * V)) : Prop :=
+  forall x y y', In (x,y) ps -> In (x,y') ps -> y = y'.
+
+Lemma functional_tail {K V} {p : K * V} {qs} :
+  functional (p :: qs) -> functional qs.
+Proof.
+  intros Hfunc k v v' Hin Hin'.
+  eapply Hfunc; right; eauto.
+Qed.
