src/Util/Show.v
@@ -1,0 +1,71 @@
+Require Import Ascii.
+Open Scope char.
+
+Require Import String.
+Require List.
+Open Scope string_scope.
+
+Class Show (X : Type) : Type := {
+  show : X -> string;
+  show_inj : forall x x', show x = show x' -> x = x'
+  }.
+
+Definition Show_dec {X} `{Show X} : forall x x' : X,
+  {x = x'} + {x <> x'}.
+Proof.
+  intros.
+  destruct (string_dec (show x) (show x')).
+  - left; now apply show_inj.
+  - right; intro.
+    apply n; congruence.
+Defined.
+
+Fixpoint char_free (c : ascii) (str : string) : Prop :=
+  match str with
+  | EmptyString => True
+  | String c' str' => c <> c' /\ char_free c str'
+  end.
+
+Lemma char_free_split : forall {c s t u v},
+  char_free c s ->
+  char_free c t ->
+  char_free c u ->
+  char_free c v ->
+  s ++ (String c t) = u ++ (String c v) ->
+  s = u /\ t = v.
+Proof.
+  intros c s.
+  induction s; intros.
+  - destruct u.
+    + inversion H3; now split.
+    + simpl in *.
+      now inversion H3.
+  - destruct u.
+    + simpl in *.
+      inversion H3.
+      now rewrite H5 in H.
+    + simpl in *.
+      inversion H3.
+      destruct H, H1.
+      destruct (IHs _ _ _ H4 H0 H7 H2 H6).
+      split; [congruence|auto].
+Qed.
+
+Class CommaFree (X : Type) `{Show X} := {
+  comma_free : forall x, char_free (",")%char (show x)
+  }.
+
+Global Instance Show_Prod {X Y} `{CommaFree X, CommaFree Y} : Show (X * Y).
+Proof.
+  apply (Build_Show _
+    (fun '(x,y) => show x ++ "," ++ show y)).
+  intros [x y] [x' y'] pair_eq.
+  inversion pair_eq.
+  destruct (char_free_split
+    (comma_free x)
+    (comma_free y)
+    (comma_free x')
+    (comma_free y') H4).
+  rewrite (show_inj _ _ H3).
+  now rewrite (show_inj _ _ H5).
+Defined.
