src/Util/StringMap.v
@@ -1,0 +1,242 @@
+Require Import Lia.
+Require Import List.
+Import ListNotations.
+Require Import String.
+
+Require Import Games.Util.Dec.
+Require Import Games.Util.Show.
+Require Games.Util.AssocList.
+
+Module AL := AssocList.
+
+Class StringMap (M : Type -> Type) : Type := {
+  empty {X} : M X;
+  add {X} : string -> X -> M X -> M X;
+  lookup {X} : string -> M X -> option X;
+  size {X} : M X -> nat;
+
+  lookup_empty {X} : forall str, lookup str (empty : M X) = None;
+  lookup_add {X} : forall str (x : X) m, lookup str (add str x m) = Some x;
+  lookup_add_neq {X} : forall str str' (x : X) m, str <> str' ->
+    lookup str (add str' x m) = lookup str m;
+  size_empty {X} : size (empty : M X) = 0;
+  size_add {X} : forall str (x : X) m,
+    size (add str x m) =
+      match lookup str m with
+      | Some _ => size m
+      | None => S (size m)
+      end
+  }.
+
+Definition str_add {M} {X Y} `{StringMap M} `{Show X} :
+  X -> Y -> M Y -> M Y :=
+  fun x => add (show x).
+
+Definition str_lookup {M} {X Y} `{StringMap M} `{Show X} :
+  X -> M Y -> option Y :=
+  fun x => lookup (show x).
+
+Lemma str_lookup_empty {M} {X Y} `{StringMap M} `{Show X} :
+  forall x, str_lookup x (empty : M Y) = None.
+Proof.
+  intro.
+  apply lookup_empty.
+Qed.
+
+Lemma str_lookup_add {M} {X Y} `{StringMap M} `{Show X} :
+  forall (x : X) (y : Y) m, str_lookup x (str_add x y m) = Some y.
+Proof.
+  intros.
+  apply lookup_add.
+Qed.
+
+Lemma str_lookup_add_neq {M} {X Y} `{StringMap M} `{Show X} :
+  forall (x x' : X) (y : Y) m, x <> x' ->
+    str_lookup x (str_add x' y m) = str_lookup x m.
+Proof.
+  intros x x' y m Hxx'.
+  apply lookup_add_neq.
+  intro Hshow.
+  apply Hxx'.
+  now apply show_inj.
+Qed.
+
+Lemma str_size_add {M} {X Y} `{StringMap M} `{Show X} :
+  forall (x : X) (y : Y) m,
+    size (str_add x y m) =
+      match str_lookup x m with
+      | Some _ => size m
+      | None => S (size m)
+      end.
+Proof.
+  intros.
+  apply size_add.
+Qed.
+
+Fixpoint str_adds {M} {X Y} `{StringMap M} `{Show X}
+  (ps : list (X * Y)) (m : M Y) {struct ps} : M Y :=
+  match ps with
+  | [] => m
+  | (x,y) :: qs => str_adds qs (str_add x y m)
+  end.
+
+Lemma str_size_add_le {M} {X Y} `{StringMap M} `{Show X}
+  (x : X) (y : Y) : forall m : M Y,
+  size m <= size (str_add x y m).
+Proof.
+  intro.
+  rewrite str_size_add.
+  destruct str_lookup; lia.
+Qed.
+
+Lemma str_size_add_lt {M} {X Y} `{StringMap M} `{Show X}
+  : forall (m : M Y) (x : X) (y : Y),
+  str_lookup x m = None ->
+  size m < size (str_add x y m).
+Proof.
+  intros.
+  rewrite str_size_add.
+  rewrite H1.
+  lia.
+Qed.
+
+Lemma str_size_adds_le {M} {X Y} `{StringMap M} `{Show X}
+  (ps : list (X * Y)) : forall m : M Y,
+  size m <= size (str_adds ps m).
+Proof.
+  induction ps as [|[x y] qs].
+  - intro; simpl. lia.
+  - intros; simpl.
+    simpl.
+    apply (PeanoNat.Nat.le_trans _ (size (str_add x y m))).
+    + apply str_size_add_le.
+    + apply IHqs.
+Qed.
+
+Lemma str_adds_ne_pos {M} {X Y} `{StringMap M} `{Show X}
+  (ps : list (X * Y)) : forall (x : X) (y : Y),
+  In (x,y) ps -> size (str_adds ps empty) > 0.
+Proof.
+  destruct ps as [|[x' y'] qs]; intros.
+  - destruct H1.
+  - simpl.
+    pose proof (str_size_adds_le qs (str_add x' y' empty)).
+    rewrite str_size_add in H2.
+    rewrite str_lookup_empty in H2.
+    lia.
+Qed.
+
+Lemma str_size_adds {M} {X Y} `{StringMap M} `{Show X}
+  (ps : list (X * Y)) : forall m : M Y,
+  NoDup (map fst ps) ->
+  (forall x, In x (map fst ps) -> str_lookup x m = None) ->
+  size (str_adds ps m) = List.length ps + size m.
+Proof.
+  induction ps as [|[x y] qs]; intros m ndps Hpsm.
+  - reflexivity.
+  - simpl.
+    rewrite IHqs.
+    + rewrite str_size_add.
+      rewrite Hpsm.
+      * apply PeanoNat.Nat.add_succ_r.
+      * left; reflexivity.
+    + now inversion ndps.
+    + intros.
+      rewrite str_lookup_add_neq.
+      * apply Hpsm.
+        right; auto.
+      * intro Hx0x.
+        rewrite Hx0x in H1.
+        now inversion ndps.
+Qed.
+
+Global Instance string_Discrete : Discrete string := {|
+  eq_dec := string_dec
+  |}.
+
+Lemma str_lookup_adds_invert {M} {X Y} `{StringMap M} `{Show X}
+  (ps : list (X * Y)) : forall (m : M Y) (x : X) (y : Y),
+  str_lookup x (str_adds ps m) = Some y ->
+  {In (x,y) ps} + {str_lookup x m = Some y}.
+Proof.
+  induction ps as [|[x y] qs]; intros m x' y' Hx'.
+  - right. exact Hx'.
+  - simpl in Hx'.
+    destruct (IHqs _ _ _ Hx').
+    + left; now right.
+    + destruct (eq_dec (show x') (show x)).
+      * assert (x' = x) as Hx'x by now apply show_inj.
+        rewrite Hx'x in e.
+        rewrite str_lookup_add in e.
+        left; left; congruence.
+      * rewrite str_lookup_add_neq in e.
+        ** now right.
+        ** intro Hx'x.
+           now rewrite Hx'x in n.
+Defined.
+
+Lemma str_lookup_adds_nIn {M} {X Y} `{StringMap M} `{Show X} :
+  forall (ps : list (X * Y)) (x : X) m,
+    ~ In x (List.map fst ps) ->
+    str_lookup x (str_adds ps m) = str_lookup x m.
+Proof.
+  intro ps.
+  induction ps as [|[x y] qs]; intros x' m nIn.
+  - reflexivity.
+  - simpl.
+    rewrite IHqs.
+    + rewrite str_lookup_add_neq.
+      * reflexivity.
+      * intro Hxx'; apply nIn.
+        left; symmetry; exact Hxx'.
+    + intro HIn; apply nIn.
+      right; auto.
+Qed.
+
+Lemma str_lookup_adds {M} {X Y} `{StringMap M} `{Show X}
+  (ps : list (X * Y)) : forall m : M Y, AL.functional ps ->
+  forall (x : X) (y : Y), In (x,y) ps ->
+  str_lookup x (str_adds ps m) = Some y.
+Proof.
+  induction ps as [|[x y] qs]; intros m ndkeys x' y' HIn.
+  - destruct HIn.
+  - simpl in *.
+    destruct HIn.
+    + inversion H1.
+      rewrite str_lookup_adds_nIn.
+      * admit.
+      * admit.
+Admitted.
+
+
+(*
+Lemma str_lookup_adds {M} {X Y} `{StringMap M} `{Show X}
+  (ps : list (X * Y)) : forall m : M Y, NoDup (List.map fst ps) ->
+  forall (x : X) (y : Y), In (x,y) ps ->
+  str_lookup x (str_adds ps m) = Some y.
+Proof.
+  induction ps as [|[x y] qs]; intros m ndkeys x' y' HIn.
+  - destruct HIn.
+  - simpl in *.
+    inversion ndkeys.
+    destruct HIn.
+    + inversion H5.
+      rewrite str_lookup_adds_nIn.
+      * apply str_lookup_add.
+      * congruence.
+    + now apply IHqs.
+Qed.
+*)
+
+Global Instance AssocList_SM : StringMap (AL.t string) := {|
+  empty X := AL.empty;
+  add X := AL.add;
+  lookup X := AL.lookup;
+  size X := AL.size;
+
+  lookup_empty X := AL.lookup_empty;
+  lookup_add X := AL.lookup_add;
+  lookup_add_neq X := AL.lookup_add_neq;
+  size_empty X := AL.size_empty;
+  size_add X := AL.size_add;
+  |}.
